blockDAG_Type.thy
@@ -1,0 +1,33 @@
+(* 
+    Author:     Joern Kussmaul
+*)
+
+theory blockDAG_Type      
+  imports blockDAG 
+begin
+
+typedef ('a,'b) BlockDAG = "{x. blockDAG x}::('a,'b) pre_digraph set"
+  morphisms BlockDAG pre_digraph_ext
+proof
+  fix a::'a
+  let ?x = "\<lparr>verts = {a}, arcs = {}, tail = \<lambda>x. a, head =  \<lambda>x. a\<rparr>" 
+  have "blockDAG ?x" unfolding blockDAG_def blockDAG_axioms_def DAG_def DAG_axioms_def 
+  digraph_def loopfree_digraph_def loopfree_digraph_axioms_def nomulti_digraph_def 
+  nomulti_digraph_axioms_def wf_digraph_def fin_digraph_def fin_digraph_axioms_def 
+  pre_digraph.del_arc_simps
+  proof(safe,simp_all, simp add: arcs_ends_def)
+    fix u::'a fix  v::'a fix e::'d
+    have "\<not>  u \<rightarrow>\<^sup>+\<^bsub>pre_digraph.del_arc ?x e\<^esub> v " 
+      by (simp add: arcs_ends_def pre_digraph.del_arc_in) 
+    then show "u \<rightarrow>\<^sup>+\<^bsub>pre_digraph.del_arc ?x e\<^esub> v 
+    \<Longrightarrow> wf_digraph.arc ?x e (u, v) \<Longrightarrow> False" by auto
+  qed
+  then show "?x \<in> {x. blockDAG x}" by simp
+qed
+
+declare [[coercion BlockDAG]]
+
+lemma
+  "blockDAG (A::('a,'b) BlockDAG)" using BlockDAG by auto
+
+end
